End to end pipeline + correctness proof

Test/SelfHosting/Main.cs
@@ -1,51 +1,58 @@
-using System;
 using Antlr4.Runtime;
 
-namespace SelfHosting.CSharp {
-  public class SimpleVisitor : SimpleBaseVisitor<AST> {
-    public override AST VisitSeq(SimpleParser.SeqContext context) {
-      return new Seq(context.s.children.Select((s, _) => (Stmt)Visit(s)).ToList());
-    }
+namespace SelfHosting.CSharp;
 
-    public override AST VisitPrint(SimpleParser.PrintContext context) {
-      return new Print((Expr)Visit(context.e));
-    }
-
-    public override AST VisitAdd(SimpleParser.AddContext context) {
-      return new Add((Expr)Visit(context.l), (Expr)Visit(context.r));
-    }
-
-    public override AST VisitConst(SimpleParser.ConstContext context) {
-      return new Const(int.Parse(context.c.Text));
-    }
+public class SimpleVisitor : SimpleBaseVisitor<AST> {
+  public override AST VisitProg(SimpleParser.ProgContext context) {
+    return new Prog(context._s.Select((s, _) => (Stmt)Visit(s)).ToList());
   }
 
-  public class ErrorListener : BaseErrorListener
+  public override AST VisitPrint(SimpleParser.PrintContext context) {
+    return new Print((Expr)Visit(context.e));
+  }
+
+  public override AST VisitAdd(SimpleParser.AddContext context) {
+    return new Add((Expr)Visit(context.l), (Expr)Visit(context.r));
+  }
+
+  public override AST VisitConst(SimpleParser.ConstContext context) {
+    return new Const(int.Parse(context.c.Text));
+  }
+}
+
+public class ErrorListener : BaseErrorListener {
+  public void SyntaxError(
+    IRecognizer recognizer, int offendingSymbol,
+    int line, int charPositionInLine, string msg,
+    RecognitionException e)
   {
-    public void SyntaxError(IRecognizer recognizer, int offendingSymbol, int line, int charPositionInLine, string msg, RecognitionException e)
-    {
-      Console.WriteLine("{0}: line {1}/column {2} {3}", e, line, charPositionInLine, msg);
+    Console.WriteLine($"{e}:{line}:{charPositionInLine}: {msg}");
+  }
+}
+
+class Program {
+  private static AST parse(string fname) {
+    using (var fstream = new StreamReader(fname)) {
+      var lexer = new SimpleLexer(new AntlrInputStream(fstream));
+      var parser = new SimpleParser(new CommonTokenStream(lexer));
+
+      // parser.RemoveErrorListeners();
+      parser.AddErrorListener(new ErrorListener()); // add ours
+
+      var visitor = new SimpleVisitor();
+      return (Prog)visitor.Visit(parser.prog());
     }
   }
 
+  public static void Main(string[] args) {
+    Console.WriteLine("# Step 1: Parse");
+    var ast = (Prog)parse(args[0]);
+    Console.WriteLine($"cAST =\n  {ast}");
 
-  class Main {
-    AST parse(string fname) {
-      using (var fstream = new StreamReader(fname)) {
-        var lexer = new SimpleLexer(new AntlrInputStream(fstream));
-        var parser = new SimpleParser(new CommonTokenStream(lexer));
+    Console.WriteLine("\n# Step 2: Compile (using Dafny)");
+    var pp = SelfHosting.DafnyCompiler.CompileAndExport(ast);
 
-        // parser.RemoveErrorListeners();
-        parser.AddErrorListener(new ErrorListener()); // add ours
-
-        var visitor = new SimpleVisitor();
-        return (Seq)visitor.Visit(parser.seq());
-      }
-    }
-
-    void main() {
-      var ast = parse("example");
-
-    }
+    Console.WriteLine("\n# Step 3: Print (using C#)");
+    pp.ForEach(s => Console.WriteLine($"  {s}"));
   }
 }
