Test/SelfHosting/cAST.cs
@@ -1,41 +1,41 @@
-using System.Collections.Generic;
+namespace SelfHosting.CSharp;
 
-namespace SelfHosting.CSharp {
-  public class AST {} // ANTLR root
+public class AST { } // ANTLR root
 
-  public class Expr : AST {}
+public class Expr : AST { }
 
-  public class Const : Expr {
-    public int n;
-    public Const(int n) {
-      this.n = n;
-    }
+public class Const : Expr {
+  public int n;
+  public Const(int n) {
+    this.n = n;
   }
+}
 
-  public class Add : Expr {
-    public Expr e1, e2;
+public class Add : Expr {
+  public Expr e1, e2;
 
-    public Add(Expr e1, Expr e2) {
-      this.e1 = e1;
-      this.e2 = e2;
-    }
+  public Add(Expr e1, Expr e2) {
+    this.e1 = e1;
+    this.e2 = e2;
   }
+}
 
-  public class Stmt : AST {}
 
-  public class Seq : AST {
-    public List<Stmt> s;
+public class Stmt : AST { }
 
-    public Seq(List<Stmt> s) {
-      this.s = s;
-    }
+public class Print : Stmt {
+  public Expr e;
+
+  public Print(Expr e) {
+    this.e = e;
   }
+}
 
-  public class Print : Stmt {
-    public Expr e;
 
-    public Print(Expr e) {
-      this.e = e;
-    }
+public class Prog : AST {
+  public List<Stmt> s;
+
+  public Prog(List<Stmt> s) {
+    this.s = s;
   }
 }
